examples/cont/client_lemmas.v
@@ -1,9 +1,9 @@
-Require Import msl.examples.cont.language.
+Require Import language.
 Require Import msl.base.
 Require Import msl.seplog.
 Require Import msl.alg_seplog.
-Require Import msl.examples.cont.seplog.
-Require Import msl.examples.cont.lseg.
+Require Import seplogic.
+Require Import lseg.
 Require Import msl.Coqlib2.
 Require Import msl.log_normalize.
 
