examples/cont/lift_seplogic.v
@@ -1,11 +1,22 @@
-Require Import msl.examples.cont.language.
+Require Import language.
 Require Import msl.base.
 Require Import msl.seplog.
 Require Import msl.alg_seplog.
 
 Local Open Scope logic.
 
-Module Type SEMAX.
+Definition lift0 {B} (P: B) : env -> B := fun _ => P.
+Definition lift1 {A1 B} (P: A1 -> B) (f1: env -> A1) : env -> B := fun rho => P (f1 rho).
+Definition lift2 {A1 A2 B} (P: A1 -> A2 -> B) (f1: env -> A1) (f2: env -> A2): 
+   env -> B := fun rho => P (f1 rho) (f2 rho).
+
+Definition subst' {A} (x: var) (e: env -> adr) (P: env -> A) : env -> A := fun s => subst x (e s) P s.
+
+Definition neq {A} (x y: A) := ~(x=y).
+Definition local {A}{NA: NatDed A} (P: env -> Prop) : env -> A := fun s => prop (P s).
+
+
+Module Type SEMAX_LIFT.
 
   Parameter mpred : Type.
   Parameter Nm: NatDed mpred.  Existing Instance Nm.
@@ -51,43 +62,44 @@ Definition funassert (G: funspecs) : mpred :=
       inlist id (map (@fst adr (list var * control)) fs) = false ->
       list_nodups vars = true ->
       length vars = length (fst P) ->
-      semax vars G (fun s => call P (map s vars)) f ->
+(*      semax vars G (fun s => call P (map s vars)) f -> *)
+      semax vars G (lift1 (call P) (fun s => map s vars)) f ->
       semax_func G fs G' ->
       semax_func G ((id, (vars,f))::fs) ((id, P) :: G').
 
   Definition program_proved (p: program) :=
    exists G, semax_func G p G 
-                            /\ table_get G 0 = Some  (0::nil, fun s => allocpool (eval (Var 0) s)).
+                            /\ table_get G 0 = Some  (0::nil, lift1 allocpool (eval (Var 0))).
 
   Axiom semax_sound: 
   forall p, program_proved p -> forall n, run p n <> None.
 
   Axiom semax_go:  forall vars G (P: funspec) x ys,   
     typecheck vars (Go x ys) = true ->
-    semax vars G (fun s => cont P (eval x s) && call P (eval_list ys s)) (Go x ys) .
+    semax vars G (lift1 (cont P) (eval x) && lift1 (call P) (eval_list ys)) (Go x ys) .
 
 Axiom semax_assign: forall x y c vars G P,
     expcheck vars y = true ->
     semax (vs_add x vars) G P c -> 
-    semax vars G (fun s => |> subst x (eval y s) P s) (Do x := y ; c). 
+    semax vars G (|> subst' x (eval y) P) (Do x := y ; c). 
 
 Axiom semax_if: forall x c1 c2 vars G (P: assert),
     expcheck vars x = true ->
-    semax vars G (fun s => !!(eval x s <> 0) && P s) c1 ->
-    semax vars G (fun s => !! (eval x s = 0) && P s) c2 ->
+    semax vars G (local (lift2 neq (eval x) (lift0 0)) && P) c1 ->
+    semax vars G (local (lift2 eq (eval x) (lift0 0)) && P) c2 ->
     semax vars G P (If x Then c1 Else c2).
 
 Axiom semax_load:  forall x y z c vars G P,
     expcheck vars y = true ->
     semax (vs_add x vars) G P c -> 
-    semax vars G (fun s => (mapsto (eval y s) z * TT) && |> subst x z P s)
+    semax vars G ((lift2 mapsto (eval y) (lift0 z) * TT) && |> subst' x (lift0 z) P)
                (Do x := Mem y ; c).
 
 Axiom semax_store: forall x y v c vars G (P: assert),
     expcheck vars x = true ->
     expcheck vars y = true ->
-    semax vars G (fun s => mapsto (eval x s) (eval y s) * P s) c ->
-    semax vars G (fun s => mapsto (eval x s) v  * P s)  (Do Mem x  := y ; c).
+    semax vars G (lift2 mapsto (eval x) (eval y) * P) c ->
+    semax vars G (lift2 mapsto (eval x) (lift0 v)  * P)  (Do Mem x  := y ; c).
 
 Axiom semax_pre: 
   forall P P' vars G c, (forall s, P s |-- P' s) -> semax vars G P' c -> semax vars G P c.
@@ -95,24 +107,25 @@ Axiom semax_pre:
 Axiom semax_exp: forall A vars G (P: A -> assert) c,
     typecheck vars c = true ->
     (forall v:A, semax vars G (P v) c) ->
-    semax vars G (fun s => EX v:A, (P v s)) c.
+    semax vars G (EX v:A, (P v)) c.
 
 Axiom semax_exp': forall A (any: A) vars G (P: A -> assert) c,
     (forall v:A, semax vars G (P v) c) ->
-    semax vars G (fun s => EX v:A, (P v s)) c.
+    semax vars G (EX v:A, (P v)) c.
 
 Axiom semax_prop:
   forall (R: Prop) vars G P c,
       typecheck vars c = true ->
       (R -> semax vars G P c) ->
-      semax vars G (fun s => !! R && P s) c.
+      semax vars G (!!R && P) c.
 
 Axiom semax_G:
-   forall vars G P c, semax vars G (fun s => P s && funassert G) c -> semax vars G P c.
+   forall vars G P c, semax vars G (P && lift0 (funassert G)) c -> semax vars G P c.
 
+End SEMAX_LIFT.
 
-End SEMAX.
-
+Require Import seplogic.
+Module S2 (Module S2: SEMAX) : SEMAX_LIFT := S2.
 
 
    
